$\sum{k} = \frac{n\times (n+1)}{2}$\\
$\sum{2k-1} = n^{2}$\\
$\sum{k^{2}} = \frac{n\times (n+1)\times (2n+1)}{6}$\\
$\sum{(2k-1)^{2}} = \frac{n\times (4n^{2}-1)}{3}$\\
$\sum{k^{3}} = (\frac{n\times (n+1)}{2})^{2}$\\
$\sum{(2k-1)^{3}} = n^{2}\times (2n^{2}-1)$\\
$\sum{k^{4}} = \frac{n\times (n+1)\times (2n+1)\times (3n^{2}+3n-1)}{30}$\\
$\sum{k^{5}} = \frac{n^{2}\times (n+1)^{2}\times (2n^{2}+2n-1)}{12}$\\
$\sum{k\times (k+1)} = \frac{n\times (n+1)\times (n+2)}{3}$\\
$\sum{k\times (k+1)\times (k+2)} = \frac{n\times (n+1)\times (n+2)\times (n+3)}{4}$\\
$\sum{k\times (k+1)\times (k+2)\times (k+3)} = \frac{n\times (n+1)\times (n+2)\times (n+3)\times (n+4)}{5}$\\
